proof/old_system/uni/algo_worklist/prop_basic.v
@@ -16,6 +16,8 @@ Proof.
   intros. induction H; auto.
 Qed.
 
+
+
 (* Fixpoint subst_tvar_in_aworklist *)
 
 (* Theorem a_wl_red_rename_tvar : forall Γ1 Γ2 X b X',
@@ -89,12 +91,16 @@ end.
 
 
 Ltac solve_notin_eq X :=
-  repeat
+  let H := fresh "H" in 
+    assert (H: X `notin` singleton X) by auto;
+    apply notin_singleton_1 in H; contradiction.
+
+  (* repeat
     match goal with 
     | H : X `notin` singleton X |- _ => apply notin_singleton_1 in H; contradiction
     | H : X `notin` singleton X `union` ?L |- _ => apply notin_union_1 in H; apply notin_singleton_1 in H; contradiction
     | H : X `notin` ?L1 `union` ?L2 |- _ => apply notin_union_2 in H
-    end.
+    end. *)
 
 
 Lemma rename_tvar_in_aworklist_fresh_eq : forall X X' Γ,
@@ -145,47 +151,69 @@ Ltac _apply_IH_a_wl_red :=
 
 Lemma worklist_subst_rename : forall Γ X1 X2 X' A E Γ1 Γ2,
   ⊢ᵃ Γ ->
-  X' `notin` ftvar_in_typ A `union` ftvar_in_aworklist' Γ ->
+  X' `notin` ftvar_in_typ A `union` ftvar_in_aworklist' Γ `union` singleton X2 ->
   aworklist_subst Γ X2 A E Γ1 Γ2 -> 
   aworklist_subst (rename_tvar_in_aworklist X' X1 Γ) (if X2 == X1 then X' else X2) ({` X' /ᵗ X1} A) 
       (rename_tvar_in_etvar_list X' X1 E) (rename_tvar_in_aworklist X' X1 Γ1) (rename_tvar_in_aworklist X' X1 Γ2).
 Proof with auto with Hdb_a_wl_red_basic.
   intros. induction H1; try solve [simpl; eauto with Hdb_a_wl_red_basic].
-  - simpl in *. dependent destruction H. destruct (X == X1)...
+  - simpl in *. destruct (X == X1).
+    + subst.
+      constructor...
+      apply IHaworklist_subst; auto.
+      dependent destruction H...
+    + constructor...
+      apply IHaworklist_subst...
+      dependent destruction H...
   - simpl in *.  _apply_IH_a_wl_red...  unfold eq_dec in *.
     destruct (EqDec_eq_of_X Y X1); destruct (EqDec_eq_of_X X X1).
-    + subst. constructor. apply IHaworklist_subst... 
+    + subst. contradiction.
+    + subst. constructor... 
       rewrite subst_tvar_in_typ_fresh_eq...
-    + subst. constructor. apply IHaworklist_subst... 
-      rewrite subst_tvar_in_typ_fresh_eq...
-    + subst. constructor. apply IHaworklist_subst...
+    + subst. constructor...
       rewrite ftvar_in_typ_subst_tvar_in_typ_upper...
-    + constructor. apply IHaworklist_subst...
+    + constructor... 
       rewrite ftvar_in_typ_subst_tvar_in_typ_upper...
   - simpl in *.  _apply_IH_a_wl_red... unfold eq_dec in *.
     destruct (EqDec_eq_of_X Y X1); destruct (EqDec_eq_of_X X X1).
-    + subst. constructor. apply IHaworklist_subst...
+    + subst. contradiction. 
+    + subst. constructor...
       rewrite subst_tvar_in_typ_fresh_eq...
-    + subst. constructor. apply IHaworklist_subst... 
-      rewrite subst_tvar_in_typ_fresh_eq...
-    + subst. constructor. apply IHaworklist_subst...
+    + subst. constructor... 
       rewrite ftvar_in_typ_subst_tvar_in_typ_upper...
-    + constructor. apply IHaworklist_subst...
+    + constructor... 
       rewrite ftvar_in_typ_subst_tvar_in_typ_upper...
   - simpl in *. _apply_IH_a_wl_red... 
   - simpl in *. _apply_IH_a_wl_red... unfold eq_dec in *.
     destruct (EqDec_eq_of_X Y X1); destruct (EqDec_eq_of_X X X1).
-    + subst. constructor. apply IHaworklist_subst... 
+    + subst. contradiction.
+    + subst. constructor... 
       rewrite subst_tvar_in_typ_fresh_eq...
-    + subst. constructor. apply IHaworklist_subst... 
-      rewrite subst_tvar_in_typ_fresh_eq...
-    + subst. constructor. apply IHaworklist_subst... 
+    + subst. constructor... 
       rewrite ftvar_in_typ_subst_tvar_in_typ_upper...
-    + constructor. apply IHaworklist_subst...
+    + constructor... 
       rewrite ftvar_in_typ_subst_tvar_in_typ_upper...
-  - simpl in *. _apply_IH_a_wl_red... 
+  - simpl in *. _apply_IH_a_wl_red... unfold eq_dec in *.
+      destruct (EqDec_eq_of_X Y X1); destruct (EqDec_eq_of_X X X1).
+      + subst. contradiction.
+      + subst. constructor...
+      + subst. constructor... 
+      + constructor... 
 Qed.
 
+
+Lemma a_mono_typ_rename : forall Γ A X X',
+  a_mono_typ (awl_to_aenv Γ) A ->
+  a_mono_typ (awl_to_aenv (rename_tvar_in_aworklist X' X Γ)) ({` X' /ᵗ X} A).
+Proof.
+  intros. dependent induction H; simpl; eauto with Hdb_a_wl_red_basic.
+  - destruct (X0 == X); constructor.
+    + subst. admit.
+    + admit.
+  - destruct (X0 == X); constructor.
+    + subst. admit.
+    + admit.
+Admitted.
 
 Lemma binds_var_typ_rename : forall x A X X' Γ,
   ⊢ᵃ Γ ->
@@ -206,6 +234,196 @@ Proof with auto with Hdb_a_wl_red_basic.
   - dependent destruction H. simpl in *...
 Qed.
 
+Lemma ftvar_in_work_apply_cont_eq : forall w A c,
+  apply_cont c A w ->
+  ftvar_in_work w [=] ftvar_in_typ A `union` ftvar_in_cont c.
+Proof.
+  intros. induction H; simpl; fsetdec.
+Qed.
+
+Lemma a_wf_wl_apply_cont : forall Γ w A c,
+  apply_cont c A w ->
+  a_wf_wl (work_apply c A ⫤ Γ) ->
+  a_wf_wl (w ⫤ Γ).
+Proof with eauto with Hdb_a_wl_red_basic.
+  intros. induction H; destruct_a_wf_wl...
+Qed.
+
+
+Lemma a_wf_wl_wf_bind_typ : forall Γ x A,
+  ⊢ᵃ Γ ->
+  binds x (abind_var_typ A) (awl_to_aenv Γ) ->
+  a_wf_typ (awl_to_aenv Γ) A.
+Proof.
+Admitted.
+
+
+Lemma tvar_notin_awl_notin_bind_typ : forall X Γ x A,
+  ⊢ᵃ Γ ->
+  X `notin` ftvar_in_aworklist' Γ ->
+  binds x (abind_var_typ A) (awl_to_aenv Γ) ->
+  X `notin` ftvar_in_typ A.
+Proof.
+Admitted.
+
+Lemma awl_app_rename_tvar_comm : forall Γ1 Γ2 X X',
+  awl_app (rename_tvar_in_aworklist X' X Γ2) (rename_tvar_in_aworklist X' X Γ1) =
+  rename_tvar_in_aworklist X' X (awl_app Γ2 Γ1).
+Proof. 
+  intros. induction Γ2; simpl in *; auto; rewrite IHΓ2; auto.
+Qed.
+
+Lemma rename_tvar_in_aworklist_rename_tvar_in_etvar_list : forall X X' E,
+  rename_tvar_in_aworklist X' X (etvar_list_to_awl E) = etvar_list_to_awl (rename_tvar_in_etvar_list X' X E).
+Proof.
+  induction E; auto.
+  - simpl. rewrite IHE. auto.
+Qed. 
+
+Lemma subst_tvar_in_typ_rename : forall X X' A B,
+  X' `notin` ftvar_in_typ A ->
+  {` X' /ᵗ X} {B /ᵗ X} A = {({` X' /ᵗ X} B) /ᵗ X'} {` X' /ᵗ X} A.
+Proof.
+  intros. induction A; simpl; auto.
+  - destruct (X0 == X); auto.
+    + simpl. unfold eq_dec. destruct (EqDec_eq_of_X X' X'); auto.
+      contradiction.
+    + simpl. unfold eq_dec. destruct (EqDec_eq_of_X X0 X).
+      * subst. contradiction.
+      * destruct (EqDec_eq_of_X X0 X').
+        subst. solve_notin_eq X'.
+        auto.
+  - simpl in *. 
+    rewrite IHA1; auto.
+    rewrite IHA2; auto.
+  - simpl in *.
+    rewrite IHA; auto.
+  - simpl in *.
+    rewrite IHA1; auto.
+    rewrite IHA2; auto.
+  - simpl in *.
+    rewrite IHA1; auto.
+    rewrite IHA2; auto.
+Qed.
+
+
+Lemma subst_tvar_in_exp_rename : forall X X' e A,
+  X' `notin` ftvar_in_exp e ->
+  (subst_tvar_in_exp ` X' X (subst_tvar_in_exp A X e)) =
+  (subst_tvar_in_exp ({` X' /ᵗ X} A) X' (subst_tvar_in_exp ` X' X e))
+with subst_tvar_in_body_rename : forall X X' b A,
+  X' `notin` ftvar_in_body b ->
+  (subst_tvar_in_body ` X' X (subst_tvar_in_body A X b)) =
+  (subst_tvar_in_body ({` X' /ᵗ X} A) X' (subst_tvar_in_body ` X' X b)).
+Proof.
+  - intros. induction e; simpl in *; auto.
+    + rewrite IHe; auto.
+    + rewrite IHe1; auto.
+      rewrite IHe2; auto.
+    + erewrite subst_tvar_in_body_rename; auto.
+    + rewrite IHe; auto.
+      rewrite subst_tvar_in_typ_rename; auto.
+    + rewrite IHe; auto.
+      rewrite subst_tvar_in_typ_rename; auto.
+  - intros. induction b.
+    simpl in *.
+    erewrite subst_tvar_in_exp_rename; auto.
+    rewrite subst_tvar_in_typ_rename; auto.
+Qed.
+
+
+Lemma subst_tvar_in_cont_rename : forall X X' A c,
+  X' `notin` ftvar_in_cont c ->
+  {` X' /ᶜₜ X} {A /ᶜₜ X} c = {({` X' /ᵗ X} A) /ᶜₜ X'} {` X' /ᶜₜ X} c.
+Proof.
+  intros. induction c; simpl in *;
+    try repeat rewrite subst_tvar_in_typ_rename; auto; 
+    try rewrite subst_tvar_in_exp_rename; auto;
+    try rewrite IHc; auto.
+Qed.
+  
+Lemma subst_tvar_in_work_rename : forall X X' w A,
+  X' `notin` ftvar_in_work w ->
+  {` X' /ʷₜ X} {A /ʷₜ X} w = {({` X' /ᵗ X} A) /ʷₜ X'} {` X' /ʷₜ X} w.
+Proof.
+  intros. destruct w; simpl in *; 
+    try repeat rewrite subst_tvar_in_typ_rename; auto; 
+    try rewrite subst_tvar_in_exp_rename; auto;
+    try rewrite subst_tvar_in_cont_rename; auto.
+Qed.
+
+
+Lemma subst_tvar_in_awl_rename_tvar_comm_eq : forall Γ X X' A,
+  X' `notin` ftvar_in_aworklist' Γ ->
+  (rename_tvar_in_aworklist X' X (subst_tvar_in_aworklist A X Γ)) =
+  (subst_tvar_in_aworklist ({` X' /ᵗ X} A) X' (rename_tvar_in_aworklist X' X Γ)).
+Proof. 
+  intros. induction Γ; simpl in *; auto; rewrite IHΓ; auto.
+  - apply f_equal. destruct ab; auto.
+    + simpl. rewrite subst_tvar_in_typ_rename; auto.
+  - apply f_equal. 
+    + destruct ab; auto.
+      * simpl. rewrite subst_tvar_in_typ_rename; auto.
+  - apply f_equal. 
+    + rewrite subst_tvar_in_work_rename; auto. 
+Qed.
+
+Lemma subst_tvar_in_awl_rename_tvar_comm_neq : forall Γ X1 X2 X' A,
+  X' <> X2 ->
+  X1 <> X2 ->
+  (rename_tvar_in_aworklist X' X1 (subst_tvar_in_aworklist A X2 Γ)) =
+  (subst_tvar_in_aworklist ({` X' /ᵗ X1} A) X2 (rename_tvar_in_aworklist X' X1 Γ)).
+Proof. 
+  intros. induction Γ; simpl in *; auto; rewrite IHΓ; auto.
+  - apply f_equal. rewrite subst_tvar_in_abind_subst_tvar_in_abind; auto.
+  - apply f_equal. rewrite subst_tvar_in_abind_subst_tvar_in_abind; auto.
+  - apply f_equal. rewrite subst_tvar_in_work_subst_tvar_in_work; auto.
+Qed.
+
+Lemma a_wf_wl_worklist_subst : forall Γ X A E Γ1 Γ2,
+  ⊢ᵃ Γ ->
+  binds X abind_etvar_empty (awl_to_aenv Γ) ->
+  aworklist_subst Γ X A E Γ1 Γ2 ->
+  ⊢ᵃ awl_app (subst_tvar_in_aworklist A X Γ2)
+     (awl_app (etvar_list_to_awl E) Γ1).
+Proof.
+  intros. induction H1; auto.
+  - dependent destruction H; auto.
+  - simpl. inversion H0; auto.
+    + dependent destruction H2.
+    + constructor; auto.
+      admit.
+      admit.
+      apply IHaworklist_subst; auto.
+      admit. 
+  - simpl. inversion H0; auto.
+      + dependent destruction H4.
+      + constructor; auto.
+        admit.
+        apply IHaworklist_subst; auto.
+        admit.
+  - simpl. inversion H0; auto.
+    + dependent destruction H4.
+    + constructor; auto.
+      admit.
+      apply IHaworklist_subst; auto.
+      admit.
+  - simpl in *. constructor.
+    admit.
+    apply IHaworklist_subst; auto.
+    admit.
+  - simpl in *. inversion H0.
+    + dependent destruction H4. contradiction.
+    + constructor.
+      admit.
+      apply IHaworklist_subst; auto.
+      admit.
+  - simpl in *. inversion H0.
+    + dependent destruction H3. contradiction.
+    + admit.
+Admitted.
+
+
 Theorem a_wl_red_rename_tvar : forall Γ X X',
   ⊢ᵃ Γ -> 
   X' `notin` ftvar_in_aworklist' Γ ->
@@ -213,15 +431,15 @@ Theorem a_wl_red_rename_tvar : forall Γ X X',
   (rename_tvar_in_aworklist X' X Γ) ⟶ᵃʷ⁎⋅.
 Proof with eauto with Hdb_a_wl_red_basic.
   intros. dependent induction H1; try solve [simpl in *; try _apply_IH_a_wl_red; eauto with Hdb_a_wl_red_basic].
-  - admit.
+  - simpl in *. destruct (X0 == X); _apply_IH_a_wl_red... 
   - simpl.
     dependent destruction H.
     eapply a_wl_red__sub_alll with (L:=L `union` singleton X `union` singleton X').
-    + admit.
-    + admit.
-    + admit.
+    + apply neq_all_rename...
+    + apply neq_intersection_rename... 
+    + apply neq_union_rename...
     + intros. simpl in *. inst_cofinites_with X0.
-      assert (⊢ᵃ (work_sub (B1 ^ᵗ X0) A1 ⫤ aworklist_constvar Γ X0 abind_etvar_empty)) by admit. 
+      assert (⊢ᵃ (work_sub (B1 ^ᵗ X0) A1 ⫤ X0 ~ᵃ ⬒;ᵃ Γ)) by admit. 
       rewrite typ_subst_open_comm...
       unfold eq_dec in H6.
       destruct (EqDec_eq_of_X X0 X) in H6...
@@ -236,7 +454,7 @@ Proof with eauto with Hdb_a_wl_red_basic.
     rewrite typ_subst_open_comm...
     unfold eq_dec in H2.
     destruct (EqDec_eq_of_X X0 X) in H2...
-    + subst. admit.
+    + subst. solve_notin_eq X. 
     + apply H2. admit.
       repeat rewrite ftvar_in_typ_open_typ_wrt_typ_upper...
   - simpl. 
@@ -253,67 +471,86 @@ Proof with eauto with Hdb_a_wl_red_basic.
       inst_cofinites_with X1. inst_cofinites_with X2.
       admit.
   - admit.
-  - simpl in *. 
-    eapply worklist_subst_rename with (X':=X') (X1:=X) in H3 as Hsubst.
-    destruct (X0 == X); apply a_wl_red__sub_etvarmono1 with (E:=rename_tvar_in_etvar_list X' X E)
-    (Γ1:=rename_tvar_in_aworklist X' X Γ1) (Γ2:=rename_tvar_in_aworklist X' X Γ2)...
+  - simpl in *. destruct_a_wf_wl.
+    eapply worklist_subst_rename with (X':=X') (X1:=X) in H5 as Hsubst...
+    unfold eq_dec in *. destruct (EqDec_eq_of_X X0 X);
+      apply a_wl_red__sub_etvarmono1 with (E:=rename_tvar_in_etvar_list X' X E)
+        (Γ1:=rename_tvar_in_aworklist X' X Γ1) (Γ2:=rename_tvar_in_aworklist X' X Γ2)...
+    + admit.
+    + apply a_mono_typ_rename...  
+    + subst.
+      rewrite <- awl_app_rename_tvar_comm in IHa_wl_red.
+      rewrite <- awl_app_rename_tvar_comm in IHa_wl_red.
+      rewrite subst_tvar_in_awl_rename_tvar_comm_eq in IHa_wl_red; auto.
+      rewrite rename_tvar_in_aworklist_rename_tvar_in_etvar_list in IHa_wl_red.
+      apply IHa_wl_red; auto.
+      admit.
+      admit.
+      admit.
+    + admit.
+    + apply a_mono_typ_rename...
+    + rewrite <- awl_app_rename_tvar_comm in IHa_wl_red.
+      rewrite <- awl_app_rename_tvar_comm in IHa_wl_red.
+      rewrite subst_tvar_in_awl_rename_tvar_comm_neq in IHa_wl_red; auto.
+      rewrite rename_tvar_in_aworklist_rename_tvar_in_etvar_list in IHa_wl_red.
+      apply IHa_wl_red; auto.
+      * admit. (* wf *)
+      * admit. 
+  - simpl in *. destruct_a_wf_wl.
+    eapply worklist_subst_rename with (X':=X') (X1:=X) in H5 as Hsubst...
+    unfold eq_dec in *. destruct (EqDec_eq_of_X X0 X); 
+      apply a_wl_red__sub_etvarmono2 with (E:=rename_tvar_in_etvar_list X' X E)
+        (Γ1:=rename_tvar_in_aworklist X' X Γ1) (Γ2:=rename_tvar_in_aworklist X' X Γ2)...
+    + admit.
+    + apply a_mono_typ_rename...  
     + admit.
     + admit.
+    + apply a_mono_typ_rename...
     + admit.
-    + admit.
-    + admit.
-    + admit.
-    + admit.
-    + admit. 
-  - simpl. 
-    eapply worklist_subst_rename with (X':=X') (X1:=X) in H3 as Hsubst.
-    destruct (X0 == X); apply a_wl_red__sub_etvarmono2 with (E:=rename_tvar_in_etvar_list X' X E)
-    (Γ1:=rename_tvar_in_aworklist X' X Γ1) (Γ2:=rename_tvar_in_aworklist X' X Γ2)...
-    + admit.
-    + admit.
-    + admit.
-    + admit.
-    + admit.
-    + admit.
-    + admit.
-    + admit. 
   - simpl in *. 
     inst_cofinites_for a_wl_red__chk_absarrow. intros.
     inst_cofinites_with x.
-    assert (⊢ᵃ (work_check (open_exp_wrt_exp e (exp_var_f x)) A2 ⫤ aworklist_consvar Γ x (abind_var_typ A1))) by admit.
-    apply H2 in H4.
-    rewrite subst_tvar_in_exp_open_exp_wrt_exp in H4...
-    admit.
-  - admit.
+    rewrite subst_tvar_in_exp_open_exp_wrt_exp in H2...
+    apply H2.
+    + admit. (* wf *)
+    + repeat rewrite ftvar_in_exp_open_exp_wrt_exp_upper...
+  - simpl in *. admit.
   - simpl in *. 
     inst_cofinites_for a_wl_red__chk_abstop. intros.
     inst_cofinites_with x.
-    assert (⊢ᵃ (work_check (open_exp_wrt_exp e (exp_var_f x)) typ_top ⫤ aworklist_consvar Γ x (abind_var_typ typ_bot))) by admit.
-    apply H2 in H4.
-    rewrite subst_tvar_in_exp_open_exp_wrt_exp in H4...
-    repeat rewrite ftvar_in_exp_open_exp_wrt_exp_upper...
+    rewrite subst_tvar_in_exp_open_exp_wrt_exp in H2...
+    apply H2.
+    + admit. (* wf *)
+    + repeat rewrite ftvar_in_exp_open_exp_wrt_exp_upper...
   - simpl in *.
-    assert (⊢ᵃ (work_apply c A ⫤ Γ)) by admit.
     dependent destruction H.
+    apply a_wf_wl_wf_bind_typ in H2 as Hwfa...
+    assert (⊢ᵃ (work_apply c A ⫤ Γ)) by now destruct_a_wf_wl; eauto with Hdb_a_wl_red_basic.
     apply IHa_wl_red in H4.
     eapply a_wl_red__inf_var with (A:=({` X' /ᵗ X} A))...
     apply binds_var_typ_rename...
-    admit.
+    apply tvar_notin_awl_notin_bind_typ with (X:=X') in H2...
   - simpl in *.
     inst_cofinites_for  a_wl_red__inf_tabs...
     intros. inst_cofinites_with X0.
-    assert (⊢ᵃ (work_check (open_exp_wrt_typ e ` X0) (A ^ᵗ X0) ⫤ X0 ~ᵃ □ ;ᵃ work_apply c (typ_all A) ⫤ Γ)) by admit.
-    apply H2 in H4.
-    rewrite subst_tvar_in_exp_open_exp_wrt_typ in H4...
-    simpl in H4.
-    rewrite <- typ_subst_open_comm in H4...
-    unfold eq_dec in H4.
-    destruct (EqDec_eq_of_X X0 X) in H4...
+    rewrite subst_tvar_in_exp_open_exp_wrt_typ in H2...
+    simpl in H2.
+    rewrite <- typ_subst_open_comm in H2...
+    unfold eq_dec in H2.
+    destruct (EqDec_eq_of_X X0 X) in H2...
     + subst. solve_notin_eq X. 
-    + admit.
+    + apply H2.
+      * admit. (* wf *)
+      * rewrite ftvar_in_exp_open_exp_wrt_typ_upper.
+        rewrite ftvar_in_typ_open_typ_wrt_typ_upper...
   - simpl in *.  
-    eapply a_wl_red__inf_abs_mono.
-    admit.
+    inst_cofinites_for a_wl_red__inf_abs_mono. 
+    intros. inst_cofinites_with x. inst_cofinites_with X1. inst_cofinites_with X2.
+    unfold eq_dec in *. destruct (EqDec_eq_of_X X2 X); destruct (EqDec_eq_of_X X1 X);
+      try solve [subst; solve_notin_eq X].
+    + rewrite subst_tvar_in_exp_open_exp_wrt_exp in H2. apply H2.
+      * admit. (* wf *)
+      * rewrite ftvar_in_exp_open_exp_wrt_exp_upper... 
   - simpl in *. 
     inst_cofinites_for a_wl_red__infabs_all.
     intros. inst_cofinites_with X0.
@@ -321,18 +558,22 @@ Proof with eauto with Hdb_a_wl_red_basic.
     unfold eq_dec in H2.
     destruct (EqDec_eq_of_X X0 X) in H2...
     + subst. solve_notin_eq X.
-    + apply H2.  admit. 
+    + apply H2.  
+      admit. (* wf *) 
       rewrite ftvar_in_typ_open_typ_wrt_typ_upper...
-  - admit.
+  - simpl in *.
+    admit.
   - simpl in *. 
-    assert ( ⊢ᵃ (work_apply c (A ^^ᵗ B) ⫤ Γ)) by admit.
-    apply IHa_wl_red in H2.
     eapply a_wl_red__inftapp_all.
     rewrite <- subst_tvar_in_typ_open_typ_wrt_typ...
-    rewrite ftvar_in_typ_open_typ_wrt_typ_upper...
-  - simpl. 
-    assert (⊢ᵃ (w ⫤ Γ)) by admit.
-    apply IHa_wl_red in H3.
-    eapply apply_cont_rename with (X:=X) (X':=X') in H1...
-    admit.
+    apply IHa_wl_red.
+    + admit.
+    + rewrite ftvar_in_typ_open_typ_wrt_typ_upper...
+  - simpl in *.
+    eapply apply_cont_rename with (X:=X) (X':=X') in H1 as Hac...
+    eapply a_wl_red__applycont; eauto.
+    apply IHa_wl_red.
+    eapply a_wf_wl_apply_cont in H; eauto.
+    + apply ftvar_in_work_apply_cont_eq in H1...
+      fsetdec.
 Admitted.
